fixtures/TypeChecker.mli
@@ -1674,6 +1674,9 @@ val check_env_root_shadow_no_receiver_component_local_bounds_narrow_summary_prov
 val check_env_root_shadow_no_receiver_component_ready_body_or_local_narrow_summary_provider_check :
   global_env -> bool
 
+val check_env_root_shadow_no_receiver_component_ready_body_or_local_narrow_summary_provider_check_with_shadow_checks :
+  global_env -> bool
+
 val check_env_root_shadow_no_receiver_component_ready_body_summary_provider_check_with_shadow_checks :
   global_env -> bool
 
